theories/core/utp_recursion.thy
@@ -1,0 +1,154 @@
+(******************************************************************************)
+(* Project: Unifying Theories of Programming in HOL                           *)
+(* File: utp_recursion.thy                                                    *)
+(* Author: Simon Foster and Frank Zeyda, University of York (UK)              *)
+(******************************************************************************)
+
+header {* Predicate Lattice *}
+
+theory utp_recursion
+imports 
+  utp_lattice
+begin
+
+subsection {* Fixed Points *}
+
+abbreviation WFP ::
+  "'VALUE WF_FUNCTION \<Rightarrow>
+   'VALUE WF_PREDICATE" ("\<mu>") where
+"WFP \<equiv> lfp"
+
+syntax
+  "_WFP" :: "pttrn => 'VALUE WF_PREDICATE => 'VALUE WF_PREDICATE" ("(3MU _./ _)" [0, 10] 10)
+
+syntax (xsymbols)
+  "_WFP" :: "pttrn => 'VALUE WF_PREDICATE => 'VALUE WF_PREDICATE" ("(3\<mu>_\<bullet>/ _)" [0, 10] 10)
+
+translations
+  "MU x. P" == "CONST WFP (%x. P)"
+
+abbreviation SFP ::
+  "'VALUE WF_FUNCTION \<Rightarrow>
+   'VALUE WF_PREDICATE" ("\<nu>") where
+"SFP \<equiv> gfp"
+
+syntax
+  "_SFP" :: "pttrn => 'VALUE WF_PREDICATE => 'VALUE WF_PREDICATE" ("(3NU _./ _)" [0, 10] 10)
+
+syntax (xsymbols)
+  "_SFP" :: "pttrn => 'VALUE WF_PREDICATE => 'VALUE WF_PREDICATE" ("(3\<nu>_\<bullet>/ _)" [0, 10] 10)
+
+translations
+  "NU x. P" == "CONST SFP (%x. P)"
+
+lemma WFP: "F(Y) \<sqsubseteq> Y \<Longrightarrow> \<mu> F \<sqsubseteq> Y"
+  by (metis lfp_lowerbound)
+
+lemma WFP_unfold: "mono F \<Longrightarrow> \<mu> F = F(\<mu> F)"
+  by (metis lfp_unfold)
+
+lemma WFP_id: "(\<mu> X \<bullet> X) = true"
+  by (metis bot_WF_PREDICATE_def bot_unique WFP)
+
+lemma SFP: "S \<sqsubseteq> F(S) \<Longrightarrow> S \<sqsubseteq> \<nu> F"
+  by (metis gfp_upperbound)
+
+lemma SFP_unfold: "mono F \<Longrightarrow> F (\<nu> F) = \<nu> F"
+  by (metis gfp_unfold)
+
+lemma SFP_id: "(\<nu> X \<bullet> X) = false"
+  by (metis SFP top_WF_PREDICATE_def top_unique)
+
+type_synonym 'a WF_PRED_CHAIN = "nat \<Rightarrow> 'a WF_PREDICATE"
+
+definition chain :: "'a WF_PRED_CHAIN \<Rightarrow> bool" where
+  "chain Y = ((Y 0 = false) \<and> (\<forall>i. Y (Suc i) \<sqsubseteq> Y i))"
+
+lemma chain0 [simp]: "chain Y \<Longrightarrow> Y 0 = false"
+  by (simp add:chain_def)
+
+lemma chainI: "\<lbrakk> Y 0 = false; \<And>i. Y (Suc i) \<sqsubseteq> Y i \<rbrakk> \<Longrightarrow> chain Y"
+  unfolding chain_def by fast
+
+lemma chainE: "\<lbrakk> chain Y; \<And> i. \<lbrakk> Y 0 = false; Y (Suc i) \<sqsubseteq> Y i \<rbrakk> \<Longrightarrow> P \<rbrakk> \<Longrightarrow> P"
+  unfolding chain_def by fast
+
+lemma L274: "\<forall> n. (E n \<and>p X = E n \<and>p Y) \<Longrightarrow> \<Sqinter> (range E) \<and>p X = \<Sqinter> (range E) \<and>p Y"
+  by (utp_pred_auto_tac)
+
+definition constr :: 
+  " ('a WF_PREDICATE \<Rightarrow> 'a WF_PREDICATE) 
+  \<Rightarrow> 'a WF_PRED_CHAIN \<Rightarrow> bool" where
+"constr F E \<longleftrightarrow> (\<forall> X n. (F(X) \<and>p E (n + 1) = F(X \<and>p E n) \<and>p E (n + 1)))"
+
+text {* This lemma gives a way of showing that there is a unique fixed-point when
+        the predicate function can be built using a constructive function F
+        over an approximation chain E *}
+lemma chain_pred_terminates: 
+  assumes "constr F E" "chain E" "mono F"
+  shows "\<Sqinter> (range E) \<and>p \<mu> F  = \<Sqinter> (range E) \<and>p \<nu> F"
+proof -
+  from assms have "\<forall> n. E n \<and>p \<mu> F = E n \<and>p \<nu> F"
+  proof (rule_tac allI)
+    fix n
+    from assms show "E n \<and>p \<mu> F = E n \<and>p \<nu> F"
+    proof (induct n)
+      case 0 thus ?case by (simp add:eval)
+    next
+      case (Suc n) 
+      note hyp = this
+      thus ?case
+      proof -
+        thm hyp
+        have "E (n + 1) \<and>p \<mu> F = E (n + 1) \<and>p F (\<mu> F)"
+          by (metis WFP_unfold assms(3))
+        
+        also from hyp have "... = E (n + 1) \<and>p F (E n \<and>p \<mu> F)"
+          by (metis (no_types) AndP_comm constr_def)
+        
+        also from hyp have "... = E (n + 1) \<and>p F (E n \<and>p \<nu> F)"
+          by simp
+        
+        also from hyp have "... = E (n + 1) \<and>p \<nu> F"
+          by (smt AndP_comm SFP_unfold constr_def)
+        
+        ultimately show ?thesis
+          by simp
+      qed
+    qed
+  qed
+    
+  thus ?thesis
+    apply (rule_tac L274)
+    apply (simp)
+  done
+qed
+
+lemma WFP_rec: 
+  assumes "(C \<Rightarrow>p S) \<sqsubseteq> F (C \<Rightarrow>p S)" "taut ([C \<Rightarrow>p (\<mu> F \<Leftrightarrow>p \<nu> F)]p)" 
+  shows "(C \<Rightarrow>p S) \<sqsubseteq> \<mu> F"
+proof -
+
+  from assms have "(C \<Rightarrow>p S) \<sqsubseteq> \<nu> F"
+    by (auto intro:SFP)
+
+  with assms show ?thesis
+    by (utp_pred_auto_tac)
+qed
+
+text {* Relational Iteration (Kleene Star) *}
+
+instantiation WF_PREDICATE :: (VALUE) star
+begin
+
+definition star_WF_PREDICATE :: "'a WF_PREDICATE \<Rightarrow> 'a WF_PREDICATE" where
+"star_WF_PREDICATE p = \<Sqinter> {p\<^bsup>n\<^esup> | n. n \<in> UNIV}"
+
+instance ..
+
+end
+
+definition IterP :: "'a WF_PREDICATE \<Rightarrow> 'a WF_PREDICATE \<Rightarrow> 'a  WF_PREDICATE" where
+"IterP b P \<equiv> \<mu> X \<bullet> ((P ; X) \<triangleleft> b \<triangleright> II)"
+
+end
