theories/core/utp_wp.thy
@@ -1,0 +1,66 @@
+theory utp_wp
+  imports utp_laws utp_lattice utp_recursion
+begin
+
+ML {*
+  structure wp =
+    Named_Thms (val name = @{binding wp} val description = "weakest precondition theorems")
+*}
+
+setup wp.setup
+
+definition WeakPrecondP :: 
+  "'VALUE WF_PREDICATE \<Rightarrow> 'VALUE WF_PREDICATE \<Rightarrow> 'VALUE WF_PREDICATE" (infixr "wp" 150) where
+"Q wp r \<equiv> \<not>p (Q ; (\<not>p r))"
+
+declare WeakPrecondP_def [eval,evalr]
+
+lemma ConjP_wp [wp]:
+  "P wp (q \<and>p r) = (P wp q) \<and>p (P wp r)"
+  by (metis (no_types) SemiP_OrP_distl WeakPrecondP_def demorgan1 demorgan2)
+
+lemma SemiR_wp [wp]: 
+  "(P ; Q) wp r = P wp (Q wp r)"
+  apply (simp add: WeakPrecondP_def)
+  apply (metis NotP_NotP SemiP_assoc)
+done
+
+lemma CondP_wp [wp]:
+  "\<lbrakk> UNREST DASHED_TWICE P; UNREST DASHED b;  UNREST DASHED_TWICE b;
+     UNREST DASHED_TWICE Q; UNREST DASHED_TWICE r \<rbrakk> \<Longrightarrow>
+  (P \<triangleleft> b \<triangleright> Q) wp r = (P wp r) \<triangleleft> b \<triangleright> (Q wp r)"
+  apply (subgoal_tac "UNREST DASHED_TWICE (\<not>p r)")
+  apply (simp add: WeakPrecondP_def SemiR_CondR_distr)
+  apply (utp_pred_auto_tac)
+  apply (blast intro:unrest)
+done
+
+lemma OrP_wp [wp]:
+  "(P \<or>p Q) wp r = (P wp r) \<and>p (Q wp r)"
+  by (metis (no_types) SemiP_OrP_distr WeakPrecondP_def demorgan1)
+
+lemma ChoiceP_wp [wp]:
+  "(P \<sqinter> Q) wp r = (P wp r) \<and>p (Q wp r)"
+  by (simp add:inf_WF_PREDICATE_def wp)
+
+lemma ImpliesP_precond_wp: "[r \<Rightarrow>p s]p \<Longrightarrow> [(Q wp r) \<Rightarrow>p (Q wp s)]p"
+  by (metis ConjP_wp RefP_def le_iff_sup less_eq_WF_PREDICATE_def sup_WF_PREDICATE_def)
+
+lemma ImpliesP_pred_wp: "[Q \<Rightarrow>p S]p \<Longrightarrow> [(S wp r) \<Rightarrow>p (Q wp r)]p"
+  by (metis OrP_comm OrP_wp RefP_def inf_WF_PREDICATE_def le_iff_inf le_iff_sup less_eq_WF_PREDICATE_def sup_WF_PREDICATE_def)
+
+lemma RefineP_precond_wp: "[r \<Rightarrow>p s]p \<Longrightarrow> Q wp s \<sqsubseteq> Q wp r"
+  by (metis ImpliesP_precond_wp RefP_def less_eq_WF_PREDICATE_def)
+
+lemma RefineP_pred_wp: "S \<sqsubseteq> Q \<Longrightarrow> Q wp r \<sqsubseteq> S wp r"
+  by (metis ChoiceP_wp inf_absorb2 le_iff_sup sup_WF_PREDICATE_def)
+
+lemma FalseP_wp: "Q ; true = true \<Longrightarrow> Q wp false = false"
+  by (simp add:WeakPrecondP_def)
+
+lemma weakest_prespec:
+  "(P ; Q) \<Rightarrow>p S = P \<Rightarrow>p (Q wp S)"
+  apply (simp add:WeakPrecondP_def)
+oops
+
+end
